A reference sheet of exponent and logarithm rules useful in constructing systems of thermal, gravitational, orbital, and energetic relationships in scientifically-grounded worldbuilding.

---

## ğŸ”¢ Rules of Exponents

### â• Product & Quotient Rules
$$
x^m \cdot x^n = x^{m+n}, \qquad \frac{x^m}{x^n} = x^{m-n}
$$

---

### ğŸ“ Index Rule
$$
\sqrt[n]{x} = x^{\frac{1}{n}}, \qquad \sqrt[-n]{x} = \frac{1}{\sqrt[n]{x}} = x^{-\frac{1}{n}}
$$

$$
\sqrt[m]{\frac{x^n}{x^p}} = x^{\frac{n - p}{m}}, \qquad \sqrt[m]{x^n x^p} = x^{\frac{n + p}{m}}
$$

---

### ğŸ” Power Rule
$$
(x^m)^n = x^{mn}, \qquad (x^{-m})^n = x^{-mn}
$$

$$
\sqrt[n]{\sqrt[m]{x}} = \sqrt[nm]{x}, \qquad \sqrt[n]{x^{\frac{1}{m}}} = x^{\frac{1}{nm}}
$$

---

### ğŸ§® Power of a Fraction
$$
\left(\frac{x}{y}\right)^n = \frac{x^n}{y^n}
$$

---

### ğŸ¯ Fractional Exponents
$$
\sqrt[m]{x^n} = x^{\frac{n}{m}}, \qquad \sqrt[n]{x^m} = x^{\frac{m}{n}}, \qquad (\sqrt[m]{x})^n = x^{\frac{n}{m}}
$$

---

### ğŸš« Negative Exponent Rule
$$
x^{-n} = \frac{1}{x^n}
$$

---

### ğŸ•³ï¸ Zero Exponent Rule
$$
x^0 = 1 \quad \text{(for } x \ne 0\text{)}
$$

---

### â™¾ï¸ Infinity Exponent Rule
$$
x^\infty = \infty, \qquad x^{-\infty} = 0
$$

---

## ğŸ§  Additional Useful Identities

### ğŸ§© Distributive Rule for Exponents over Multiplication
$$
(xy)^n = x^n y^n, \qquad \left(\frac{x}{y}\right)^n = \frac{x^n}{y^n}
$$

---

### ğŸ”„ Logarithmic Inverses
$$
\log_b(b^x) = x, \qquad b^{\log_b(x)} = x
$$

---

### ğŸªœ Logarithmic Expansion Rules
$$
\log(xy) = \log x + \log y, \qquad \log\left(\frac{x}{y}\right) = \log x - \log y, \qquad \log(x^n) = n \log x
$$

---

### ğŸŒ€ Reciprocal Roots
$$
\sqrt[n]{\frac{1}{x}} = \frac{1}{\sqrt[n]{x}} = x^{-\frac{1}{n}}
$$

---

### ğŸ“ˆ Arbitrary Exponentials in Terms of *e*
$$
a^x = e^{x \ln a}
$$

---

## ğŸ“Š Powers and Logs
$$
x^y = z \quad \Rightarrow \quad y = \frac{\log z}{\log x} = \log_x z
$$

$$
x = z^{\frac{1}{y}} = \sqrt[y]{z}
$$


# ğŸ§® General-Use Equations

### ğŸ“˜ Variable Definitions
- **u** = upper bound  
- **l** = lower bound  
- **s** = sum of bounds (total)  
- **d** = difference between bounds (span)  
- **r** = ratio of lower to upper bound  
- **m** = mean (average)  
- **p** = product of bounds  
- **q** = quotient of bounds  

## ğŸ“ Number Relationships
### â— Ratio
$$
\text{ratio} = \frac{l}{u} = \frac{\text{sum} - \text{difference}}{\text{sum} + \text{difference}}
$$

---

### â• Sum & Difference Identities
$$
\text{sum} = u + l = d\left(1 + \frac{1}{r}\right), \qquad
\text{difference} = u - l = s\left(\frac{1 - r}{1 + r}\right)
$$

---

### ğŸ”€ Transformations Between Bounds
$$
l = \frac{s - d}{2}, \qquad
u = \frac{s + d}{2}, \qquad
s = l + u, \qquad
d = u - l
$$

---

### ğŸ” Alternate Forms with Ratio
$$
l = \frac{s}{1 + r}, \qquad
u = \frac{rs}{1 + r}
$$

$$
l = s \cdot \left(\frac{1}{1 + r}\right), \qquad
u = s \cdot \left(\frac{r}{1 + r}\right)
$$

$$
l = \frac{s - d}{2}, \qquad
u = \frac{s + d}{2}, \qquad
l = \frac{(s - d) \cdot r}{1 + r}, \qquad
u = \frac{s \cdot r + d}{1 + r}
$$

---

### ğŸ“Š Mean
$$
m = \frac{u + l}{2}, \qquad
m = \frac{s}{2}, \qquad
m = u - \frac{d}{2}, \qquad
m = l + \frac{d}{2}
$$

---

### ğŸ§® Inequality Notes
$$
m \gg \frac{1}{2} u \quad \text{(if } u < 0 \text{ and } l > 0\text{)}
$$

$$
m = \frac{1}{2} u \quad \text{(if } l = 0\text{)}
$$

$$
m = u = l \quad \text{(if } u = l\text{)}
$$

---

### âœ–ï¸ Product & Quotient
$$
\text{Product } = xy = \frac{s^2 - d^2}{4}
$$

$$
\text{Quotient } = \frac{x + d}{x - d} = \frac{(x + y) + (x - y)}{(x + y) - (x - y)}
$$

$$
\frac{s}{d} = \frac{x + y}{x - y}, \qquad \frac{d}{s} = \frac{x - y}{x + y}
$$

---

## ğŸ“‰ Percentage from Portion
### ğŸ”¢ Percentage (p) from portion (x) of total  (n)

$$
p = \frac{x}{n}, \qquad x = pn, \qquad n = \frac{p}{x}
$$

---

### ğŸ“˜ Definitions
- **p** = percentage  
- **x** = portion (part)  
- **n** = base number (whole)
## ğŸ¯ Percentages in Ranges
### ğŸ“ Percentage (p) Represented by a Value (v) in Range (l â€¦ u)
$$
p = \frac{v - l}{u - l}, \qquad v = p(u - l) + l, \qquad u = \frac{v - l}{p} + l, \qquad l = \frac{v - pu}{1 - p}
$$

#### ğŸ”¤ Variable Definitions
- **v** = value within the range  
- **l** = lower bound  
- **u** = upper bound  
- **p** = percentage of the \([l, u]\) range represented by \(v\)

---

### ğŸ” Transfer a Percentage Between Two Ranges
#### ğŸ§® General Equations
Let:
- \( R_1 = [\text{min}, \text{num}, \text{max}] \)
- \( R_2 = [z, x, y] \), where \( x < z < y \)

Then:
$$
\text{pct} = \frac{\text{num} - \text{min}}{\text{max} - \text{min}}, \qquad
z = \text{pct} \cdot (y - x) + x
$$

---

#### âœ… Example
Given:
- \( R_1 = [0, 6, 10] \)
- \( R_2 = [4, z, 6] \)

Then:
$$
\text{pct} = \frac{6 - 0}{10 - 0} = \frac{6}{10} = 0.60
$$

$$
z = 0.60 \cdot (6 - 4) + 4 = 0.60(2) + 4 = 5.2
$$

Check:
$$
\frac{5.2 - 4}{6 - 4} = \frac{1.2}{2} = 0.60
$$

---

## ğŸ”¢ Sums of Number Sequences

### ğŸ“˜ Variable Definitions
- **Î£** = sum of all integers in the range (l â€¦ u)  
- **s** = sum of bounds: \( u + l \)  
- **d** = difference: \( u - l \)  
- **l** = lower bound of range  
- **u** = upper bound of range  

### â• Consecutive Integers from (l â€¦  u)
$$
s = u + l, \qquad d = u - l
$$

#### ğŸ§® Summation Formulas
Basic:
$$
\Sigma = \frac{u(u + 1)}{2} - \frac{l(l - 1)}{2}
$$

Symmetric:
$$
\Sigma = \frac{l^2 - 1}{2} + \frac{u^2 + u}{2}, \qquad
\Sigma = \frac{(u + l)(u - l + 1)}{2}
$$

Sum in terms of \( d \) and \( s \):
$$
\Sigma = \frac{d + 1}{2} s, \qquad
\Sigma = \frac{sd + s}{2}
$$

Expanded forms:
$$
\Sigma = \frac{u^2 + u}{2} - \frac{l^2 - l}{2}
$$

$$
\Sigma = \frac{(u^2 + u) - (l^2 - l)}{2}, \qquad
\Sigma = \frac{u^2 - l^2 + u + l}{2}, \qquad
\Sigma = \frac{u^2 - l^2 + s}{2}
$$

---

## ğŸ”¢ Integer Sequences and Special Transformations

### ğŸŸ¥ Consecutive Odd Integers (1 â€¦ u)
$$
\Sigma_o = \left( \frac{u + 1}{2} \right)^2 = \frac{u^2 + 2u + 1}{4}
$$

---

### ğŸŸ¦ Consecutive Even Integers (2 â€¦ u)
$$
\Sigma_e = \left( \frac{u}{2} \right) \left( \frac{u}{2} + 1 \right) = \frac{u(u + 2)}{4} = \frac{u^2 + 2u}{4}
$$

---

### ğŸ§® Count of Consecutive Integers in Range (1 â€¦ u)
$$
\left\lfloor \frac{u - l}{2} \right\rfloor + 1 \quad \text{for odd or even spacing}
$$

or for total count of integers:
$$
\left\lfloor \frac{u - l}{2} \right\rfloor \cdot 2 + 1 = 2\left\lfloor \frac{u - l}{2} \right\rfloor + 1
$$

---

### ğŸ“‰ Percent Difference

$$
\%\Delta = 100 \cdot \frac{\text{new} - \text{old}}{\text{old}} = 100 \left( \frac{\text{new}}{\text{old}} - 1 \right)
$$

---

### ğŸ” Involutive Transformation
Given:
$$
y = \frac{1 - x}{1 + x}
$$

Then:
$$
x = \frac{1 - y}{1 + y}
$$

This is its own inverse: \( f(f(x)) = x \)

---

### ğŸ”„ Percentage Inversion (Reciprocal Percentages)
If $x\% \text{ of } y = y\% \text{ of } x$, then:

$$
\frac{x}{100} \cdot y = \frac{y}{100} \cdot x, \qquad
x \cdot \frac{y}{100} = y \cdot \frac{x}{100}
$$

---

## ğŸŸ¨ Generalized Metallic Mean for Any Integer $x$
The traditional formula is:

$$
N_x = \frac{x + \sqrt{x^2 + 4}}{2}
$$

This generalizes the golden ratio (\(x = 1\)), silver ratio (\(x = 2\)), bronze ratio (\(x = 3\)), etc.

Alternative equivalent form:
$$
N_x = \sqrt{1 + \frac{x^2}{4}} + \frac{x}{2}
$$

This version is symmetric and may be more intuitive in nested radical systems.

---

## ğŸ“ˆ Pointâ€“Slope of a Line
Given two points:

$$
\begin{gather}
P_1 = (x_1, y_1) \\[6pt]
P_2 = (x_2, y_2)
\end{gather}
$$

---

### ğŸ§® Slope Formula
$$
m = \frac{y_1 - y_2}{x_1 - x_2}
$$

---

### ğŸ§¾ Pointâ€“Slope Form
$$
y - y_1 = m(x - x_1)
$$

Or rearranged:
$$
y = m(x - x_1) + y_1
$$

---

### ğŸ¯ Slopeâ€“Intercept Form
$$
y = mx + b
$$

---

### ğŸ”ƒ Converting from Pointâ€“Slope to Slopeâ€“Intercept
$$
\begin{align}
\text{Start with pointâ€“slope:} \quad & y - y_1 = m(x - x_1) \\[6pt]
\text{Distribute the slope:} \quad & y = mx - mx_1 + y_1 \\[6pt]
\text{Group constants:} \quad & y = mx + (y_1 - mx_1) \\[6pt]
\text{Therefore:} \quad & b = y_1 - mx_1
\end{align}
$$

> ğŸ§  **Note:** The subscripts vanish because their values get absorbed into the constant \( b \).  
> The slopeâ€“intercept form still â€œremembersâ€ your point â€” just more subtly.

---

## ğŸ§ª Example 1
Given:  
- \( P_1 = (4.85, 0) \)  
- \( P_2 = (1, 1) \)

### Step 1: Find the slope
$$
m = \frac{0 - 1}{4.85 - 1} = \frac{-1}{3.85}
$$

### Step 2: Use pointâ€“slope form
$$
y - 0 = \frac{-1}{3.85}(x - 4.85)
$$

### Step 3: Rearrange to slopeâ€“intercept form
$$
y = \frac{-1}{3.85}x + \frac{4.85}{3.85} \approx -0.26x + 1.26
$$

---

## ğŸ§ª Example 2
Given:  
- \( P_1 = (0.5, 0) \)  
- \( P_2 = (1, 1) \)

### Step 1: Find the slope
$$
m = \frac{0 - 1}{0.5 - 1} = \frac{-1}{-0.5} = 2
$$

### Step 2: Use pointâ€“slope form
$$
y - 0 = 2(x - 0.5)
$$

### Step 3: Rearrange to slopeâ€“intercept form
$$
y = 2x - 1
$$

![[Line Point-Slope Illustration.png|500]]

## ğŸ“‰ Visualizing Pointâ€“Slope Examples

This plot shows the two lines derived in the examples above:

- **Blue Line**:  
  From $P_1 = (4.85, 0)$ and $P_2 = (1, 1)$  
  $y = -0.25974x + 1.25974$

- **Red Line**:  
  From $P_1 = (0.5, 0)$ and $P_2 = (1, 1)$  
  $y = 2x - 1$

They intersect at the point (1, 1), which lies on both lines.

---

## ğŸŒ¡ï¸ Temperature Scale Equalities
### ğŸ” Fahrenheit â†” Kelvin
**Core conversion equations:**
$$
C = K - 273.15, \qquad C = \frac{5}{9}(F - 32)
$$

So:
$$
K - 273.15 = \frac{5}{9}(F - 32)
$$

Or rearranged:
$$
K = \frac{5}{9}(F - 32) + 273.15
$$

And:
$$
F = \frac{9}{5}(K - 273.15) + 32
$$

---

### ğŸ§ª Worked Example (Convert 255.372 K to Â°F)
Start from:
$$
K = 255.372
$$

Plug into conversion formula:
$$
K - 273.15 = \frac{5}{9}(F - 32)
$$

$$
-17.7778 = \frac{5}{9}(F - 32)
$$

Multiply both sides by 9:
$$
-160 = 5(F - 32)
$$

Divide by 5:
$$
-32 = F - 32
$$

So:
$$
F = 0^\circ\text{F}
$$

Alternatively, in reverse:
$$
F = 0 \Rightarrow K = \frac{5}{9}(0 - 32) + 273.15 = -17.7778 + 273.15 = 255.372 \text{ K}
$$

---

### ğŸŒ¡ï¸ Fahrenheit â†” Celsius
Standard conversion formulas:
$$
F = \frac{9}{5}C + 32, \qquad C = \frac{5}{9}(F - 32)
$$

#### ğŸ” Rearrangements:
From:
$$
F = \frac{9}{5}C + 32
$$

Subtract 32:
$$
F - 32 = \frac{9}{5}C
$$

Multiply both sides by 5:
$$
5(F - 32) = 9C
$$

Divide by 9:
$$
C = \frac{5}{9}(F - 32)
$$

### ğŸ§ª Worked Example (Convert -40Â°F to Â°C)
$$
C = \frac{5}{9}(-40 - 32) = \frac{5}{9}(-72) = -40
$$

So:
$$
-40^\circ \text{F} = -40^\circ \text{C}
$$
### ğŸŒ¡ï¸ Kelvin â†” Celsius
The Kelvin and Celsius scales are offset by a constant:
$$
K = C + 273.15, \qquad C = K - 273.15
$$

> ğŸ“ **Note:** The size of 1 degree is identical in both scales; only the zero point differs.
> Water freezes at 0â€¯Â°C = 273.15â€¯K and boils at 100â€¯Â°C = 373.15â€¯K.

> ğŸ“ **Terminology Note:**  
> Temperatures on the Kelvin scale are written simply as **K**, without a degree symbol.  
> For example:  
> - Correct:â€ƒ**273.15 K**  âœ“
> - Incorrect:â€ƒ**273.15â€¯Â°K** â€“ or â€“ **273.15 degrees Kelvin**
